Semantics.thy
@@ -1,8 +1,10 @@
-theory Semantics imports Syntax Utils "HOL-Library.AList" begin
+theory Semantics imports Syntax Utils begin
+
+no_notation inverse_divide (infixl "'/" 70) \<comment> \<open>avoid clash with division notation\<close>
 
 text\<open>For next meeting:
 Questions/Help:
-
+- Type freshness assumptions?
 To talk about:
 - T-Mod premise formulas use \<forall> qualifiers, which are not actually a thing in the formula syntax.
   I suppose we just "desugar" this into an AND over the finite number of set elements?
@@ -10,6 +12,7 @@ To talk about:
 - Figured out where "bit variables" appear: For chomp & heapRef. If I understand it correctly,
   chomp introduces placeholder variables into expressions, and then heapRef replaces them with
   concrete values again.
+- Should I stick with slices only even given e.g. the T-Mod rule?
 \<close>
 
 section\<open>Expressions and Formulas\<close>
@@ -218,5 +221,64 @@ where
   CS_Id:     "HT \<turnstile> (In, Out, H, c) \<rightarrow>* (In, Out, H, c)" |
   CS_Step:   "\<lbrakk> HT \<turnstile> t \<rightarrow> t''; HT \<turnstile> t'' \<rightarrow>* t' \<rbrakk>
              \<Longrightarrow> HT \<turnstile> t \<rightarrow>* t'"
+
+
+section\<open>Types\<close>
+
+(* TODO: Do these need freshness assumptions? *)
+nominal_function heap_ty_sem :: "heap_ty \<Rightarrow> env \<Rightarrow> heap set" ("\<lbrakk>_ in _\<rbrakk>\<^sub>t" [50,60] 100)
+where
+  "\<lbrakk>Nothing in \<epsilon>\<rbrakk>\<^sub>t = {}" |
+  "\<lbrakk>Top in \<epsilon>\<rbrakk>\<^sub>t = UNIV" |
+  "\<lbrakk>Sigma x \<tau>\<^sub>1 \<tau>\<^sub>2 in \<epsilon>\<rbrakk>\<^sub>t = {h\<^sub>1 ++ h\<^sub>2 | h\<^sub>1 h\<^sub>2. h\<^sub>1 \<in> \<lbrakk>\<tau>\<^sub>1 in \<epsilon>\<rbrakk>\<^sub>t \<and> h\<^sub>2 \<in> \<lbrakk>\<tau>\<^sub>2 in \<epsilon>[x \<rightarrow> h\<^sub>1]\<rbrakk>\<^sub>t}" |
+  "\<lbrakk>Choice \<tau>\<^sub>1 \<tau>\<^sub>2 in \<epsilon>\<rbrakk>\<^sub>t = \<lbrakk>\<tau>\<^sub>1 in \<epsilon>\<rbrakk>\<^sub>t \<union> \<lbrakk>\<tau>\<^sub>2 in \<epsilon>\<rbrakk>\<^sub>t" |
+  "\<lbrakk>Refinement x \<tau> \<phi> in \<epsilon>\<rbrakk>\<^sub>t = {h | h. h \<in> \<lbrakk>\<tau> in \<epsilon>\<rbrakk>\<^sub>t \<and> \<lbrakk>\<phi> in \<epsilon>[x \<rightarrow> h]\<rbrakk>\<^sub>f = Some True}" |
+  "atom x \<sharp> (\<tau>\<^sub>2, \<epsilon>) \<Longrightarrow> \<lbrakk>Substitution \<tau>\<^sub>1 x \<tau>\<^sub>2 in \<epsilon>\<rbrakk>\<^sub>t = {h | h h\<^sub>2. (h\<^sub>2 \<in> \<lbrakk>\<tau>\<^sub>2 in \<epsilon>\<rbrakk>\<^sub>t) \<and> (h \<in> \<lbrakk>\<tau>\<^sub>1 in \<epsilon>[x \<rightarrow> h\<^sub>2]\<rbrakk>\<^sub>t)}"
+  using [[simproc del: alpha_lst]]
+  subgoal by (auto simp add: eqvt_def heap_ty_sem_graph_aux_def)
+  subgoal by (erule heap_ty_sem_graph.induct) (auto)
+  apply clarify
+  subgoal for P t e
+    apply (rule heap_ty.strong_exhaust[of t P])
+    apply (auto simp add: fresh_star_def fresh_Pair)
+    sorry
+  apply (simp_all add: fresh_star_def fresh_at_base)
+  subgoal for x t2 e t1 x' t1'
+    apply (erule Abs_lst1_fcb2'[where c = "(t2, e)"])
+    apply (simp_all add: eqvt_at_def fresh_star_def)
+    apply (simp_all add: perm_supp_eq Abs_fresh_iff fresh_Pair)
+    (*apply (metis fresh_star_def fresh_star_supp_conv supp_perm_eq_test)*)
+done
+nominal_termination (eqvt)
+  by lexicographic_order
+
+thm Abs_lst1_fcb2'
+thm perm_supp_eq
+thm fresh_star_supp_conv
+thm supp_perm_eq_test
+thm fresh_Pair
+thm heap_ty.strong_exhaust
+
+(*
+  using [[simproc del: alpha_lst]]
+  subgoal by (simp add: eqvt_def subst_graph_aux_def)
+  subgoal by (erule subst_graph.induct) (auto simp: fresh_star_def fresh_at_base)
+                      apply clarify
+  subgoal for P t s y
+    by (rule term.strong_exhaust[of t P "(s, y)"]) (auto simp: fresh_star_def fresh_Pair)
+                      apply (simp_all add: fresh_star_def fresh_at_base)
+  subgoal for x' y' s' t' x t
+    apply (erule Abs_lst1_fcb2'[where c = "(s', y')"])
+       apply (simp_all add: eqvt_at_def fresh_star_def)
+       apply (simp_all add: perm_supp_eq Abs_fresh_iff fresh_Pair)
+    apply (metis fresh_star_def fresh_star_supp_conv supp_perm_eq_test)
+    apply (metis fresh_star_def fresh_star_supp_conv supp_perm_eq_test)
+    done
+  done
+
+*)
+
+
+
 
 end
